1. $(x^2 - 2xy)dy=(xy-y^2)dx$ [–†–µ—à–µ–Ω–∏–µ](#1)
2. $\int\limits_{-\frac{1}{7}}^{1}\frac{xdx}{\sqrt{8+2x-x^2}}$ [–†–µ—à–µ–Ω–∏–µ](#1)

# 1

![number1](img/1.png)

–î–∏—Ñ—Ñ–µ—Ä–µ–Ω—Ü–∏–∞–ª—å–Ω–æ–µ —É—Ä–∞–≤–Ω–µ–Ω–∏–µ –ø–µ—Ä–≤–æ–≥–æ –ø–æ—Ä—è–¥–∫–∞ –Ω–∞–∑—ã–≤–∞–µ—Ç—Å—è –æ–¥–Ω–æ—Ä–æ–¥–Ω—ã–º
–µ—Å–ª–∏ –æ–Ω–æ –º–æ–∂–µ—Ç –±—ã—Ç—å –ø—Ä–µ–¥—Å—Ç–∞–≤–ª–µ–Ω–æ –≤ –≤–∏–¥–µ ùë¶‚Ä≤ = ùëì(ùë•, ùë¶). –°–º. –õ–µ–∫—Ü–∏–∏ —Å—Ç—Ä. 86

# 2

$$\int\limits_{-\frac{1}{7}}^{1}\frac{xdx}{\sqrt{8+2x-x^2}} =$$
$$\int\limits_{-\frac{1}{7}}^{1}\frac{(x-1+1)dx}{\sqrt{9-(x-1)^2}} =$$
$$\int\limits_{-\frac{1}{7}}^{1}\frac{(x-1)dx}{\sqrt{9-(x-1)^2}} +\int\limits_{-\frac{1}{7}}^{1}\frac{dx}{\sqrt{9-(x-1)^2}} =$$
$$arcsin(\frac{x-1}{3}) - \sqrt{9-(x-1)^2} \Bigg|_{-\frac{1}{7}}^1$$
